Constellation/CallAtomicProcesses.lean
@@ -1,0 +1,51 @@
+import Constellation.ProcessesWithAtomic
+
+inductive Reach
+    {Name: Type}
+    {decls: Name → Process (List Name) }
+: Rel (Process (List Name)) (List Name) where
+
+  | init p:
+      Reach p []
+
+  | exec p p' l':
+      Reach   p  [] →
+      Exec (p, []) (p', l') →
+      Reach           p'  l'
+
+  | unpend p n l:
+      Reach p (n :: l) →
+      Reach (p * decls n) l
+
+def call (s: String): Process (List String) :=
+  Process.update (some ∘ List.cons s)
+
+def decls: String → Process (List String)
+  | "main" => call "main"
+  | _ => ▪
+
+section Examples
+
+  abbrev Reach' := Reach (decls := decls)
+
+  example: Reach' ▪ [] := Reach.init ▪
+
+  example: Reach' (call "main") [] := Reach.init _
+
+  example: Reach' ▪ ["main"] := by
+    apply Reach.exec (call "main")
+    . constructor
+    . constructor
+      unfold Function.comp
+      rfl
+
+end Examples
+
+-- Did not ultimately need this, turns out
+theorem exec_midstep {State: Type} {x z: Process State × State}
+    (py: Process State)
+    (σy: State)
+    (h1: Exec⊹ x (py,σy))
+    (h2: Exec⊹   (py,σy) z)
+  :      Exec⊹ x         z
+:= TransClos.midstep h1 h2
