Constellation/FunRel.lean
@@ -3,8 +3,8 @@ TODO port to using these
 
 -/
 import Mathlib.Logic.Relation
-#print Relation.ReflTransGen
-#print Relation.TransGen
+-- #print Relation.ReflTransGen
+-- #print Relation.TransGen
 
 abbrev Rel     (α β: Sort u) := α → β → Prop
 abbrev EndoRel (α  : Sort u) := Rel α α
